

• Example #20:

- Consider the first-order ODE:

$$\frac{dy}{dt} + 1y = e^{-2t}, \quad \text{with } y(0^+) = 1$$

$\begin{matrix} \text{a} & & f(t) \\ \swarrow & & \uparrow \\ \text{1} & \text{0} & \text{p} \end{matrix}$

- Determine y_{zs} , y_{zi} and $y(t)$. for $t > 0$

$$f(t) = e^{-2t} \quad (p \neq a) \Rightarrow$$

$$y_p(t) = B e^{-2t}$$

$$y_h(t) = A e^{-at} = A e^{-t}$$

① Substitute y_p into ODE:

$$\frac{dy_p}{dt} + y_p = e^{-2t}$$

$$\frac{d}{dt}(B e^{-2t}) + B e^{-2t} = e^{-2t}$$

$$-2B e^{-2t} + B e^{-2t} = e^{-2t}$$

$$-B e^{-2t} = e^{-2t}$$

$$B = -1$$

$$y(t) = -e^{-2t} + A e^{-t}$$

$$y(t) = B e^{-2t} + A e^{-t} \quad t > 0$$

• Example #20-cont:

- Consider the first-order ODE:

$$y(t) = -e^{-2t} + A e^{-t}$$

$$y(t) = \overset{\checkmark}{y_{zs}(t)} + \underbrace{y_{zi}(t)}$$

$$\frac{dy}{dt} + y = e^{-2t}, \text{ with } y(0^+) = 1$$

- Determine y_{zs} , y_{zi} and $y(t)$.

② Use I.C. to find A:

$$y(0^+) = -e^{-2(0)} + A e^{-0} = -1 + A \Rightarrow A = y(0^+) + 1$$

$$y(t) = -e^{-2t} + (y(0^+) + 1) e^{-t} = -e^{-2t} + \underbrace{y(0^+) e^{-t}}_{zI} + \underbrace{e^{-t}}_{zS}$$

$$\begin{aligned} y_{zs}(t) &= -e^{-2t} + e^{-t} \\ + y_{zi}(t) &= y(0^+) e^{-t} = e^{-t} \\ y(t) &= -e^{-2t} + e^{-t} + e^{-t} = -e^{-2t} + 2e^{-t} \quad t > 0 \end{aligned}$$

$$\cos(a+b) = \cos a \cos b - \sin a \sin b$$

$$H \cos(t+\psi) = H(\cos t \cos \psi - \sin t \sin \psi) =$$

$$= \underbrace{H \cos \psi}_{B} \cos t - \underbrace{H \sin \psi}_{D} \sin t$$

$$y_h(t) = A e^{-t}$$

• Example #21:

• Consider the first-order ODE:

$$\frac{dy}{dt} + y = \overset{f(t)}{\cos(t)}, \text{ with } y(0^+) = 1$$

$\omega = 1 \text{ rad/s}$

$$y_p(t) = \underbrace{H \cos(t+\psi)}_{= B \cos t + D \sin t} =$$

• Determine y_{zs} , y_{zi} and $y(t)$.

① Substitute y_p into ODE:

$$\frac{dy_p}{dt} + y_p = \cos t$$

$$\frac{d}{dt} (B \cos t + D \sin t) + B \cos t + D \sin t = \cos t$$

$$-B \sin t + D \cos t + B \cos t + D \sin t = \cos t$$

$$\underbrace{(-B+D)}_0 \sin t + \underbrace{(D+B)}_1 \cos t = 0 \sin t + 1 \cos t$$

$$\Downarrow D=B=\frac{1}{2}$$

$$y_p = \frac{1}{2} \cos t + \frac{1}{2} \sin t$$

$$y(t) = y_p(t) + y_h(t) = \frac{1}{2} \cos t + \frac{1}{2} \sin t + A e^{-t}$$

• Example #21-cont:

- Consider the first-order ODE:

$$\frac{dy}{dt} + y = \cos(t), \text{ with } y(0^+) = 1$$

- Determine y_{zs} , y_{zi} and $y(t)$.

② Use I.C. to find A:

$$y(0^+) = \underbrace{\frac{1}{2} \cos(0)}_1 + \underbrace{\frac{1}{2} \sin(0)}_0 + A = \frac{1}{2} + A \Rightarrow A = y(0^+) - \frac{1}{2}$$

$$y(t) = \frac{1}{2} \cos(t) + \frac{1}{2} \sin(t) + (y(0^+) - \frac{1}{2}) e^{-t}$$

$$y_{zs}(t) \text{ (} y(0^+) = 0 \text{)} = \frac{1}{2} \cos(t) + \frac{1}{2} \sin(t) - \frac{1}{2} e^{-t}$$

$$+ y_{zi}(t) = y(0^+) e^{-t} = e^{-t}$$

$$y(t) = \frac{1}{2} \cos(t) + \frac{1}{2} \sin(t) - \frac{1}{2} e^{-t} + e^{-t} \quad t \geq 0$$

• Example #22:

- Consider the particular solution:

$$y_p(t) = \underbrace{\left(\frac{1}{2}\right) \cos(t)}_B + \underbrace{\left(\frac{1}{2}\right) \sin(t)}_D = \underbrace{H \cos(t + \psi)}_{\text{?}}, =$$

- Determine H and ψ

$$= \underbrace{H \cos \psi \cos t}_B - \underbrace{H \sin \psi \sin t}_D$$

Get ψ :

$$\frac{H \sin \psi}{H \cos \psi} = \frac{-1/2}{1/2} \Rightarrow \tan \psi = -1 \Rightarrow \psi = -\frac{\pi}{4} \text{ or } \frac{3\pi}{4}$$

↓

$$H \cos \psi = \frac{1}{2}$$

$$-H \sin \psi = \frac{1}{2}$$

Get H:

$$H \cos \psi = \frac{1}{2}$$

$$H \cos(-\pi/4) = \frac{1}{2}$$

$$H = \frac{\sqrt{2}}{2} \text{ or } -\frac{\sqrt{2}}{2}$$

$$y_p(t) = \frac{\sqrt{2}}{2} \cos(t - \pi/4) =$$

$$= -\frac{\sqrt{2}}{2} \cos(t + \pi/4)$$

- Transient vs steady-state response

- *Transient response*, $y_{tr}(t)$ is such that

$$\lim_{t \rightarrow \infty} y_{tr}(t) \rightarrow 0$$

- *Steady-state response*, $y_{ss}(t)$ is what is left after $\lim_{t \rightarrow \infty} y_{tr}(t) \rightarrow 0$

$$y(t) = y_{tr}(t) + y_{ss}(t)$$

- Recall

$$y(t) = Ae^{-at} + B$$

Handwritten notes: $t \rightarrow \infty$ $y_{tr} \rightarrow 0$ $y_{ss} \rightarrow B$

$$y(t) = Ae^{-at} + Be^{-pt}$$

Handwritten notes: $t \rightarrow \infty$ $y_{tr} \rightarrow 0$ $y_{ss} \rightarrow B$

$$y(t) = Ae^{-at} + H\cos(\omega t + \psi)$$

Handwritten notes: $t \rightarrow \infty$ $y_{tr} \rightarrow 0$ $y_{ss} \rightarrow H\cos(\omega t + \psi)$